# baseURI: https://ensnare.nobatek.com/intervention#
# prefix: interv

@prefix owl: <http://www.w3.org/2002/07/owl#> .
@prefix rdf: <http://www.w3.org/1999/02/22-rdf-syntax-ns#> .
@prefix rdfs: <http://www.w3.org/2000/01/rdf-schema#> .
@prefix interv: <https://ensnare.nobatek.com/intervention#> .
@prefix bldg: <https://ensnare.nobatek.com/building#> .
@prefix proj: <https://ensnare.nobatek.com/project#> .
@prefix xsd: <http://www.w3.org/2001/XMLSchema#> .

<https://ensnare.nobatek.com/intervention#> 
    rdf:type owl:Ontology ;
    owl:versionIRI <https://ensnare.nobatek.com/intervention/0.1> ;
    <http://purl.org/dc/terms/contributor> "Pierre Bourreau" ;
    <http://purl.org/dc/terms/description> "The ENSNARE intervention ontology describes different actions that can be performed for an energy renovation. Actions are either generic (i.e. can be performed in any or in standards energy renovation programs), or ENSNARE specific (i.e. installing off-site façade modules that incorporate active energy renewable systems"@en ;
    <http://purl.org/dc/terms/title> "The ENSNARE intervention ontology"@en .

#################################################################
#    Annotation properties
#################################################################

###  http://purl.org/dc/terms/contributor
<http://purl.org/dc/terms/contributor> rdf:type owl:AnnotationProperty .


###  http://purl.org/dc/terms/description
<http://purl.org/dc/terms/description> rdf:type owl:AnnotationProperty .


###  http://purl.org/dc/terms/title
<http://purl.org/dc/terms/title> rdf:type owl:AnnotationProperty .
  
interv:InsulateFacade rdf:type proj:Recommendation_Passive;
 rdfs:comment "Renovation recommendation to insulate the façade".
    
interv:InsulateRoof rdf:type proj:Recommendation_Passive ;
 rdfs:comment "Renovation recommendation to insulate the roof".

interv:ChangeWindows rdf:type proj:Recommendation_Passive ;
 rdfs:comment "Renovation recommendation to change the windows".
    
interv:Ventilation rdf:type proj:Recommendation_Active ;
 rdfs:comment "Renovation recommendation to install or change the ventilation system".
    
interv:Heating rdf:type proj:Recommendation_Active ;
 rdfs:comment "Renovation recommendation to change the heating system".
   
interv:DomesticHotWater rdf:type proj:Recommendation_Active ;
 rdfs:comment "Renovation recommendation to change the domestic hot water system".
    
interv:InstallPV rdf:type proj:Recommendation_Active ;
 rdfs:comment "Renovation recommendation to install some PV panels".

## Facade Action

interv:RenovationAction rdf:type owl:Class ;
    rdfs:comment "A renovation action is a refinement of a recommendation. It specifies the type of product to use".


interv:ETI_PVC_15cm
  rdf:type interv:RenovationAction ;
  interv:refines interv:InsulateFacade ;
  rdfs:label "ETI PVC 15cm" ;
  rdfs:comment "External thermal insulation of the façade with a thickness of 15cm. The material used is polystyrene" ;
.
interv:ETI_PVC_10cm
  rdf:type interv:RenovationAction ;
  interv:refines interv:InsulateFacade ;
  rdfs:label "ETI PVC 10cm" ;
  rdfs:comment "External thermal insulation of the façade with a thickness of 10cm. The material used is polystyrene" ;
.
interv:ETI_PVC_5cm
  rdf:type interv:RenovationAction ;
  interv:refines interv:InsulateFacade ;
  rdfs:label "ETI PVC 5cm" ;
  rdfs:comment "External thermal insulation of the façade with a thickness of 5cm. The material used is polystyrene" ;
.
interv:ETI_PVC_44cm
  rdf:type interv:RenovationAction ;
  interv:refines interv:InsulateFacade ;
  rdfs:label "ETI PVC 44cm" ;
  rdfs:comment "External thermal insulation of the façade with a thickness of 44cm. The material used is polystyrene" ;
.
interv:ETI_PVC_30cm
  rdf:type interv:RenovationAction ;
  interv:refines interv:InsulateFacade ;
  rdfs:label "ETI PVC 30cm" ;
  rdfs:comment "External thermal insulation of the façade with a thickness of 30cm. The material used is polystyrene" ;
.
interv:ETI_PVC_20cm
  rdf:type interv:RenovationAction ;
  interv:refines interv:InsulateFacade ;
  rdfs:label "ETI PVC 20cm" ;
  rdfs:comment "External thermal insulation of the façade with a thickness of 20cm. The material used is polystyrene" ;
.
interv:ENSNARE_10cm
  rdf:type interv:RenovationAction ;
  interv:refines interv:InsulateFacade ;
  rdfs:label "ENSNARE 10cm" ;
  rdfs:comment "ENSNARE-integrated external thermal insulation of the façade with a thickness of 10cm."
.
interv:ENSNARE_20cm
  rdf:type interv:RenovationAction ;
  interv:refines interv:InsulateFacade ;
  rdfs:label "ENSNARE 20cm" ;
  rdfs:comment "ENSNARE-integrated external thermal insulation of the façade with a thickness of 20cm." ;
.
interv:ENSNARE_30cm
  rdf:type interv:RenovationAction ;
  interv:refines interv:InsulateFacade ;
  rdfs:label "ENSNARE 30cm" ;
  rdfs:comment "ENSNARE-integrated external thermal insulation of the façade with a thickness of 30cm." ;
.
#interv:ENSNARE_PVC_10cm
#  rdf:type interv:RenovationAction ;
#  interv:refines interv:InsulateFacade ;
#  rdfs:label "ENSNARE PVC 10cm" ;
#.
#interv:ENSNARE_PVC_20cm
#  rdf:type interv:RenovationAction ;
#  interv:refines interv:InsulateFacade ;
#.
#interv:ENSNARE_PVC_30cm
#  rdf:type interv:RenovationAction ;
#  interv:refines interv:InsulateFacade ;
#  rdfs:label "ENSNARE PVC 30cm" ;
#.
#interv:ENSNARE_Mineral_10cm
#  rdf:type interv:RenovationAction ;
#  interv:refines interv:InsulateFacade ;
#  rdfs:label "ENSNARE Mineral 10cm" ;
#.
#interv:ENSNARE_Mineral_20cm
#  rdf:type interv:RenovationAction ;
#  interv:refines interv:InsulateFacade ;
#  rdfs:label "ENSNARE Mineral 20cm" ;
#.
#interv:ENSNARE_Mineral_30cm
#  rdf:type interv:RenovationAction ;
#  interv:refines interv:InsulateFacade ;
#  rdfs:label "ENSNARE Mineral 30cm" ;
#.
#interv:ENSNARE_Biosourced_10cm
#  rdf:type interv:RenovationAction ;
#  interv:refines interv:InsulateFacade ;
#  rdfs:label "ENSNARE Biosourced 10cm" ;
#.
#interv:ENSNARE_Biosourced_20cm
#  rdf:type interv:RenovationAction ;
#  interv:refines interv:InsulateFacade ;
#  rdfs:label "ENSNARE Biosourced 20cm" ;
#.
#interv:ENSNARE_Biosourced_30cm
#  rdf:type interv:RenovationAction ;
#  interv:refines interv:InsulateFacade ;
#  rdfs:label "ENSNARE Biosourced 30cm" ;
#.
interv:ENSNARE_None
  rdf:type interv:RenovationAction ;
  interv:refines interv:InsulateFacade ;
  rdfs:label 'ENSNARE no insulation' ;
.

##

interv:Insulation_Roof_XPS_10cm
  rdf:type interv:RenovationAction ;
  interv:refines interv:InsulateRoof ;
  rdfs:label "Insulation Roof XPS 10cm" ;
.
interv:Insulation_Roof_XPS_15cm
  rdf:type interv:RenovationAction ;
  interv:refines interv:InsulateRoof ;
  rdfs:label "Insulation Roof XPS 15cm" ;
.
interv:Insulation_Roof_XPS_18cm
  rdf:type interv:RenovationAction ;
  interv:refines interv:InsulateRoof ;
  rdfs:label "Insulation Roof XPS 18cm" ;
.
interv:Insulation_Roof_XPS_22cm
  rdf:type interv:RenovationAction ;
  interv:refines interv:InsulateRoof ;
  rdfs:label "Insulation Roof XPS 22cm" ;
.
interv:Insulation_Roof_XPS_30cm
  rdf:type interv:RenovationAction ;
  interv:refines interv:InsulateRoof ;
  rdfs:label "Insulation Roof XPS 30cm" ;
.
interv:Insulation_Roof_XPS_45cm
  rdf:type interv:RenovationAction ;
  interv:refines interv:InsulateRoof ;
  rdfs:label "Insulation Roof XPS 45cm" ;
.
interv:Insulation_Roof_XPS_60cm
  rdf:type interv:RenovationAction ;
  interv:refines interv:InsulateRoof ;
  rdfs:label "Insulation Roof XPS 60cm" ;
.

##

interv:DoubleGlazedWindows
	rdf:type interv:RenovationAction ;
	interv:refines interv:ChangeWindows ;
	rdfs:label "double-glazed windows" ;
.
interv:ENSNARE_ClassicWindows
	rdf:type interv:RenovationAction ;
	interv:refines interv:ChangeWindows ;
	rdfs:label "wlassic windows" ;
.
interv:ENSNARE_ActiveWindows
	rdf:type interv:RenovationAction ;
	interv:refines interv:ChangeWindows, interv:Ventilation ;
	rdfs:label "active windows" ;
.

##
interv:COP
    rdf:type rdfs:DatatypeProperty ;
    rdfs:domain interv:HeatPump ;
    rdfs:label "COP - Coefficient of Performance" ;
	rdfs:range xsd:double ;
.
interv:HeatPump
    rdf:type interv:RenovationAction ;
	interv:refines interv:Heating, interv:DomesticHotWater ;
	rdfs:label "Heat Pump" ;
.
interv:CentralHeatPump
	rdfs:subClassOf interv:HeatPump ;
	rdfs:label "central heat pump" ;
	interv:COP 4.5 ;
.
interv:IndividualHeatPump
	rdfs:subClassOf interv:HeatPump ;
	rdfs:label "individual heat pump" ;
	interv:COP 4.5 ;
.
interv:DualFlowVentilation
	rdf:type interv:RenovationAction ;
	interv:refines interv:Heating, interv:Ventilation ;
	rdfs:label "dual flow ventilation" ;
.
interv:PV_Roof
  rdf:type interv:RenovationAction ;
  interv:refines interv:InstallPV ;
  rdfs:label "PV installation - Roof" ;
  interv:elecPerf 0.2 ;
.

interv:elecPerf
	rdfs:type owl:DatatypeProperty ;
	rdfs:domain interv:ENSNARE_PV, interv:ENSNARE_PVT ;
	rdfs:range xsd:double ;
	rdfs:label "electricity production performance factor" ;
.
interv:thermalPerf
	rdfs:type owl:DatatypeProperty ;
	rdfs:domain interv:ENSNARE_ST, interv:ENSNARE_PVT ;
	rdfs:range xsd:double ;
	rdfs:label "thermal production performance factor" ;
.
interv:ENSNARE_Product
	rdf:type owl:Class ;
	rdfs:label "Generic ENSNARE active product" ;
.
interv:ENSNARE_PV
	rdfs:subClassOf interv:ENSNARE_Product ;
	interv:elecPerf 0.16 ;
    rdfs:label "ENSNARE PV panel" ;
.
interv:ENSNARE_ST
	rdfs:subClassOf interv:ENSNARE_Product ;
	interv:thermalPerf 0.84;
	rdfs:label "ENSNARE solar thermal panels" ;
.
interv:ENSNARE_PVT
	rdfs:subClassOf interv:ENSNARE_Product ;
	interv:elecPerf 0.18 ;
	interv:thermalPerf 0.58 ;
	rdfs:label "ENSNARE hybrid PV+T panel" ;
.
## Inverter Performance = 0.97

interv:PV_surface 
    rdf:type rdfs:DatatypeProperty ;
    rdfs:domain interv:RenoScenario ;
	interv:product interv:ENSNARE_PV ;
    rdfs:range xsd:double ;
    rdfs:label "ENSNARE PV installation surface" ;
.
interv:ST_surface
    rdf:type rdfs:DatatypeProperty ;
    rdfs:domain interv:RenoScenario ;
	interv:thermalPerf 4.0 ;
    rdfs:range xsd:double ;
    rdfs:label "ENSNARE Solar Thermal installation surface" ;
.
interv:PVT_surface
    rdf:type rdfs:DatatypeProperty ;
    rdfs:domain interv:RenoScenario ;
	interv:elecPerf 7.2 ;
	interv:thermalPerf 2.5 ;
    rdfs:range xsd:double ;
    rdfs:label "ENSNARE PV+T installation surface" ;
.

interv:Facade_Needed_Solar rdf:type owl:Class ;
    rdfs:label "Surface needed for a solar system installation"
.
interv:Facade_needed_PV
    rdfs:subClassOf interv:Facade_Needed_Solar ;
    rdfs:label "Surface needed for a PV installation".
interv:Facade_needed_ST
    rdfs:subClassOf interv:Facade_Needed_Solar ;
    rdfs:label "Surface needed for an ST installation".
interv:Facade_needed_PVT
    rdfs:subClassOf interv:Facade_Needed_Solar ;
     rdfs:label "Surface needed for a PV+T installation".
interv:needed_surface
    rdf:type rdfs:DatatypeProperty ;
    rdfs:domain interv:Facade_Needed_Solar ;
    rdfs:range xsd:double ;
    rdfs:comment "surface needed for an active system installation" ;
.
interv:facade
    rdf:type owl:ObjectProperty ;
    rdfs:domain interv:Facade_Needed_Solar ;
    rdfs:range bldg:Facade ;
    rdfs:comment "surface distribution of the façade surface per active systems." ;
.
interv:scenario
    rdf:type owl:ObjectProperty ;
    rdfs:domain bldg:Facade ;
    rdfs:range interv:EnsnareScenario ;
    rdfs:comment "renovation of a façade as part of an ENSNARE renovatoin scenario" ;
.
