# baseURI: https://nobatek.inef4.com/data-models/renovation-scenario#
# prefix: rscen

@prefix dbo: <http://dbpedia.org/ontology/> .
@prefix dce: <http://purl.org/dc/elements/1.1/> .
@prefix dcterms: <http://purl.org/dc/terms/> .
@prefix owl: <http://www.w3.org/2002/07/owl#> .
@prefix rdf: <http://www.w3.org/1999/02/22-rdf-syntax-ns#> .
@prefix rdfs: <http://www.w3.org/2000/01/rdf-schema#> .
@prefix rscen: <https://nobatek.inef4.com/data-models/renovation-scenario#> .
@prefix schema: <https://schema.org/> .
@prefix vann: <http://purl.org/vocab/vann/> .
@prefix vcard: <http://www.w3.org/2006/vcard/ns#> .
@prefix voaf: <http://purl.org/vocommons/voaf#> .
@prefix vs: <http://www.w3.org/2003/06/sw-vocab-status/ns#> .
@prefix xsd: <http://www.w3.org/2001/XMLSchema#> .

dcterms:contributor
  rdf:type owl:AnnotationProperty ;
.
dcterms:creator
  rdf:type owl:AnnotationProperty ;
.
dcterms:description
  rdf:type owl:AnnotationProperty ;
.
dcterms:issued
  rdf:type owl:AnnotationProperty ;
.
dcterms:license
  rdf:type owl:AnnotationProperty ;
.
dcterms:modified
  rdf:type owl:AnnotationProperty ;
.
dcterms:title
  rdf:type owl:AnnotationProperty ;
.
vann:preferredNamespacePrefix
  rdf:type owl:AnnotationProperty ;
.
vann:preferredNamespaceUri
  rdf:type owl:AnnotationProperty ;
.
voaf:Vocabulary
  rdf:type owl:Class ;
.
vs:term_status
  rdf:type owl:AnnotationProperty ;
.
vcard:fn
  rdf:type owl:AnnotationProperty ;
.
rscen:
  rdf:type voaf:Vocabulary ;
  rdf:type owl:Ontology ;
  dcterms:creator "Pierre Bourreau" ;
  dcterms:description """The Renovation Scenarion Ontology (RenOnt) is designed to describe renovation scenarios, in particular those related to energy-efficient renovations.
		It characterizes Renovation Alternatives"""@en ;
  dcterms:issued "2022-10-19T12:00:00"^^xsd:dateTime ;
  dcterms:license <https://creativecommons.org/licenses/by/1.0/> ;
  dcterms:modified "2020-07-31T08:51:00"^^xsd:dateTime ;
  dcterms:title "A Renovation Scenario Ontology (RenOnt)"@en ;
  vann:preferredNamespacePrefix "rscen:" ;
  vann:preferredNamespaceUri rscen: ;
  owl:versionInfo "0.1" ;
.
rscen:AirAirHeatPumpInstallation
  rdf:type rscen:RenoAlternative ;
  rscen:refines rscen:CoolingInstallation ;
  rscen:refines rscen:HeatingInstallation ;
  rscen:refines rscen:HeatingReplacement ;
.
rscen:AirWaterHeatPumpInstallation
  rdf:type rscen:RenoAlternative ;
  rscen:refines rscen:CoolingInstallation ;
  rscen:refines rscen:HeatingInstallation ;
  rscen:refines rscen:HeatingReplacement ;
  rscen:refines rscen:HotWaterReplacement ;
.
rscen:BaselineScenario
  rdf:type owl:Class ;
  rdfs:subClassOf rscen:RenoScenario ;
.
rscen:BoilerReplacement
  rdf:type rscen:RenoAlternative ;
  rscen:refines rscen:HeatingReplacement ;
  rscen:refines rscen:HotWaterReplacement ;
.
rscen:Budget
  rdf:type rscen:FinancialConstraint ;
  rdfs:comment "The global budget of the renovation, has defined by the client. It does not entail potential incentives." ;
  rscen:value xsd:double ;
.
rscen:BuildingCharacteristics
  rdfs:comment "A specific type of generation criterion, related to the status of the building. It encompasses all kind of information related to the existing building, prior renovation." ;
  rdfs:isDefinedBy rscen: ;
  rdfs:subClassOf rscen:Criterion ;
  owl:disjointWith rscen:ClimateConditions ;
  owl:disjointWith rscen:FinancialConstraint ;
.
rscen:ClimateConditions
  rdfs:comment "A specific type of generation criterion, related to the status of the building. It encompasses all kind of information related to the existing building, prior renovation." ;
  rdfs:isDefinedBy rscen: ;
  rdfs:subClassOf rscen:Criterion ;
  owl:disjointWith rscen:BuildingCharacteristics ;
  owl:disjointWith rscen:FinancialConstraint ;
.
rscen:ClimateZone
  rdf:type rscen:ClimateConditions ;
  rdfs:comment "The climate zone where the building is located." ;
  rscen:value [
      owl:oneOf (
          "Alpine North"
          "Alpine South"
          "Atlantic North"
          "Atlantic Central"
          "Lusitanian"
          "Boreal"
          "Nemoral"
          "Continental"
          "Pannonian"
          "Anatolian"
          "Mediterranean Mountain"
          "Mediterranean North"
          "Mediterranean South"
        ) ;
    ] ;
.
rscen:CoolingInstallation
  rdf:type rscen:RenoApproach ;
.
rscen:CoolingInstalled
  rdf:type rscen:BuildingCharacteristics ;
  rdfs:comment "Flag/boolean indicating the presence of a cooling system before renovation." ;
  rscen:value "xsd:boolean" ;
.
rscen:CoolingReplacement
  rdf:type rscen:RenoApproach ;
.
rscen:Criterion
  rdf:type owl:Class ;
  rdfs:comment "A criterion is a parameter of influence in the generation of a renovation scenario." ;
  rdfs:isDefinedBy rscen: ;
  owl:disjointWith rscen:RenoAction ;
  owl:disjointWith rscen:RenoAlternative ;
  owl:disjointWith rscen:RenoApproach ;
.
rscen:DoorsReplacement
  rdf:type rscen:RenoApproach ;
.
rscen:DoubleGlazedWindowInstallation
  rdf:type rscen:RenoAlternative ;
  rscen:refines rscen:WindowsReplacement ;
.
rscen:ETI_Biosourced_10cm_Aluminium
  rdf:type rscen:RenoAction ;
  rscen:refines rscen:ExternalFaçadeInsulation ;
.
rscen:ETI_Biosourced_10cm_Coating
  rdf:type rscen:RenoAction ;
  rscen:refines rscen:ExternalFaçadeInsulation ;
.
rscen:ETI_Biosourced_10cm_PVC
  rdf:type rscen:RenoAction ;
  rscen:refines rscen:ExternalFaçadeInsulation ;
.
rscen:ETI_Biosourced_10cm_Wood
  rdf:type rscen:RenoAction ;
  rscen:refines rscen:ExternalFaçadeInsulation ;
.
rscen:ETI_Biosourced_14cm_Aluminium
  rdf:type rscen:RenoAction ;
  rscen:refines rscen:ExternalFaçadeInsulation ;
.
rscen:ETI_Biosourced_14cm_Coating
  rdf:type rscen:RenoAction ;
  rscen:refines rscen:ExternalFaçadeInsulation ;
.
rscen:ETI_Biosourced_14cm_PVC
  rdf:type rscen:RenoAction ;
  rscen:refines rscen:ExternalFaçadeInsulation ;
.
rscen:ETI_Biosourced_14cm_Wood
  rdf:type rscen:RenoAction ;
  rscen:refines rscen:ExternalFaçadeInsulation ;
.
rscen:ETI_Coating_10cm_Coating
  rdf:type rscen:RenoAction ;
  rscen:refines rscen:ExternalFaçadeInsulation ;
.
rscen:ETI_Coating_14cm_Coating
  rdf:type rscen:RenoAction ;
  rscen:refines rscen:ExternalFaçadeInsulation ;
.
rscen:ETI_Mineral_10cm_Aluminium
  rdf:type rscen:RenoAction ;
  rscen:refines rscen:ExternalFaçadeInsulation ;
.
rscen:ETI_Mineral_10cm_Coating
  rdf:type rscen:RenoAction ;
  rscen:refines rscen:ExternalFaçadeInsulation ;
.
rscen:ETI_Mineral_10cm_PVC
  rdf:type rscen:RenoAction ;
  rscen:refines rscen:ExternalFaçadeInsulation ;
.
rscen:ETI_Mineral_10cm_Wood
  rdf:type rscen:RenoAction ;
  rscen:refines rscen:ExternalFaçadeInsulation ;
.
rscen:ETI_Mineral_14cm_Aluminium
  rdf:type rscen:RenoAction ;
  rscen:refines rscen:ExternalFaçadeInsulation ;
.
rscen:ETI_Mineral_14cm_Coating
  rdf:type rscen:RenoAction ;
  rscen:refines rscen:ExternalFaçadeInsulation ;
.
rscen:ETI_Mineral_14cm_PVC
  rdf:type rscen:RenoAction ;
  rscen:refines rscen:ExternalFaçadeInsulation ;
.
rscen:ETI_Mineral_14cm_Wood
  rdf:type rscen:RenoAction ;
  rscen:refines rscen:ExternalFaçadeInsulation ;
.
rscen:ETI_PVC_10cm_Aluminium
  rdf:type rscen:RenoAction ;
  rscen:refines rscen:ExternalFaçadeInsulation ;
.
rscen:ETI_PVC_10cm_PVC
  rdf:type rscen:RenoAction ;
  rscen:refines rscen:ExternalFaçadeInsulation ;
.
rscen:ETI_PVC_10cm_Wood
  rdf:type rscen:RenoAction ;
  rscen:refines rscen:ExternalFaçadeInsulation ;
.
rscen:ETI_PVC_14cm_Aluminium
  rdf:type rscen:RenoAction ;
  rscen:refines rscen:ExternalFaçadeInsulation ;
.
rscen:ETI_PVC_14cm_PVC
  rdf:type rscen:RenoAction ;
  rscen:refines rscen:ExternalFaçadeInsulation ;
.
rscen:ETI_PVC_14cm_Wood
  rdf:type rscen:RenoAction ;
  rscen:refines rscen:ExternalFaçadeInsulation ;
.
rscen:ElectricityCons
  rdf:type rscen:BuildingCharacteristics ;
  rdfs:comment "The yearly electricity consumption of the building." ;
  rscen:value xsd:double ;
.
rscen:ExternalFaçadeInsulation
  rdf:type rscen:RenoAlternative ;
  rscen:refines rscen:InsulateFaçade ;
.
rscen:ExternalInsulation
  rdf:type rscen:BuildingCharacteristics ;
  rdfs:comment "A boolean value to determine whether an external insulation is already installed (true) or not (false)." ;
  rscen:value xsd:boolean ;
.
rscen:ExternalRoofInsulation
  rdf:type rscen:RenoAlternative ;
  rscen:refines rscen:InsulateRoof ;
.
rscen:FaçadeInsulationLevel
  rdf:type rscen:BuildingCharacteristics ;
  rdfs:comment "The level of insulation of the façade. Values are None, Low or High." ;
  rscen:value [
      owl:oneOf (
          "None"
          "Low"
          "Medium"
          "High"
        ) ;
    ] ;
.
rscen:FinancialConstraint
  rdfs:comment "A specific type of generation criterion, related to the economic constraints of the project. Typically, the global budget of the project is a driver for a renovation project." ;
  rdfs:isDefinedBy rscen: ;
  rdfs:subClassOf rscen:Criterion ;
  owl:disjointWith rscen:BuildingCharacteristics ;
  owl:disjointWith rscen:ClimateConditions ;
.
rscen:GazCons
  rdf:type rscen:BuildingCharacteristics ;
  rdfs:comment "The yearly gaz consumption of the building." ;
  rscen:value xsd:double ;
.
rscen:HeatingEnergy
  rdf:type rscen:BuildingCharacteristics ;
  rdfs:comment "The type of energy used for heating." ;
  rscen:value [
      owl:oneOf (
          "Electricity"
          "Gaz"
          "Fuel"
          "Wood"
          "Other"
        ) ;
    ] ;
.
rscen:HeatingMode
  rdf:type rscen:BuildingCharacteristics ;
  rdfs:comment "The type of heating in the building, whether it is a central or individual system." ;
  rscen:value [
      owl:oneOf (
          "Central"
          "Individual"
        ) ;
    ] ;
.
rscen:HeatingReplacement
  rdf:type rscen:RenoApproach ;
.
rscen:HotWaterReplacement
  rdf:type rscen:RenoApproach ;
.
rscen:ITI_10cm
  rdf:type rscen:RenoAction ;
  rscen:refines rscen:InternalFaçadeInsulation ;
.
rscen:ITI_14cm
  rdf:type rscen:RenoAction ;
  rscen:refines rscen:InternalFaçadeInsulation ;
.
rscen:ITI_Biosourced_10cm
  rdf:type rscen:RenoAction ;
  rscen:refines rscen:InternalFaçadeInsulation ;
.
rscen:ITI_Biosourced_14cm
  rdf:type rscen:RenoAction ;
  rscen:refines rscen:InternalFaçadeInsulation ;
.
rscen:ITI_Mineral_10cm
  rdf:type rscen:RenoAction ;
  rscen:refines rscen:InternalFaçadeInsulation ;
.
rscen:ITI_Mineral_14cm
  rdf:type rscen:RenoAction ;
  rscen:refines rscen:InternalFaçadeInsulation ;
.
rscen:InsulateFaçade
  rdf:type rscen:RenoApproach ;
.
rscen:InsulateRoof
  rdf:type rscen:RenoApproach ;
.
rscen:InsulateSlab
  rdf:type rscen:RenoApproach ;
.
rscen:InternalFaçadeInsulation
  rdf:type rscen:RenoAlternative ;
  rscen:refines rscen:InsulateFaçade ;
.
rscen:InternalRoofInsulation
  rdf:type rscen:RenoAlternative ;
  rscen:refines rscen:InsulateRoof ;
.
rscen:LEDInstallation
  rdf:type rscen:RenoAlternative ;
  rscen:refines rscen:LightingReplacement ;
.
rscen:LightingReplacement
  rdf:type rscen:RenoApproach ;
.
rscen:LoftInsulation
  rdf:type rscen:RenoAlternative ;
  rscen:refines rscen:InsulateRoof ;
.
rscen:Orientation
  rdf:type rscen:BuildingCharacteristics ;
  rdfs:comment "Orientation of the building, considering the façade with the main entrance." ;
  rscen:value [
      owl:oneOf (
          "North"
          "South"
          "West"
          "East"
        ) ;
    ] ;
.
rscen:PV-TInstallationFaçade
  rdf:type rscen:RenoAlternative ;
  rscen:refines rscen:HotWaterReplacement ;
  rscen:refines rscen:PVInstallation ;
.
rscen:PV-TInstallationRoof
  rdf:type rscen:RenoAlternative ;
  rscen:refines rscen:HotWaterReplacement ;
  rscen:refines rscen:PVInstallation ;
.
rscen:PVInstallation
  rdf:type rscen:RenoApproach ;
.
rscen:PVInstallationFaçade
  rdf:type rscen:RenoAlternative ;
  rscen:refines rscen:PVInstallation ;
.
rscen:PVInstallationRoof
  rdf:type rscen:RenoAlternative ;
  rscen:refines rscen:PVInstallation ;
.
rscen:RenoAction
  rdf:type owl:Class ;
  rdfs:comment "A renovation action is a refinement of a renovation alternative, with technical details on the elements to associate to the renovation; ex: external wall insulation with 14cm mineral wool." ;
  rdfs:isDefinedBy rscen: ;
  owl:disjointWith rscen:RenoAlternative ;
  owl:disjointWith rscen:RenoApproach ;
  owl:disjointWith rscen:RenoScenario ;
.
rscen:RenoAlternative
  rdf:type owl:Class ;
  rdfs:comment "A renovation alternative is a refinement of a renovation approach, describing into more details the type of renovation action that will be made; ex: external/internal wall insulation..." ;
  rdfs:isDefinedBy rscen: ;
  owl:disjointWith rscen:RenoAction ;
  owl:disjointWith rscen:RenoApproach ;
  owl:disjointWith rscen:RenoScenario ;
.
rscen:RenoApproach
  rdf:type owl:Class ;
  rdfs:comment "A renovation approach describes the type of work that can be executed. It must be related to a some building element/renovation post; ex: insulation, windows, doors..." ;
  rdfs:isDefinedBy rscen: ;
  owl:disjointWith rscen:RenoAction ;
  owl:disjointWith rscen:RenoAlternative ;
  owl:disjointWith rscen:RenoScenario ;
.
rscen:RenoProject
  rdf:type owl:Class ;
  rdfs:comment "A renovation project is associated to one or many buildings, and can comprise many renovation scenarios." ;
  rdfs:isDefinedBy rscen: ;
  owl:disjointWith rscen:Criterion ;
  owl:disjointWith rscen:RenoAction ;
  owl:disjointWith rscen:RenoAlternative ;
  owl:disjointWith rscen:RenoApproach ;
  owl:disjointWith rscen:RenoScenario ;
.
rscen:RenoScenario
  rdf:type owl:Class ;
  rdfs:comment "A renovation scenario is a way to envisage the renovation of a/many buildings. It is made of multiple renovation approaches." ;
  rdfs:isDefinedBy rscen: ;
  owl:disjointWith rscen:Criterion ;
  owl:disjointWith rscen:RenoAction ;
  owl:disjointWith rscen:RenoAlternative ;
  owl:disjointWith rscen:RenoApproach ;
.
rscen:RoofInsulationLevel
  rdf:type rscen:BuildingCharacteristics ;
  rdfs:comment "The level of insulation of the roof. Values are None, Low or High." ;
  rscen:value [
      owl:oneOf (
          "None"
          "Low"
          "Medium"
          "High"
        ) ;
    ] ;
.
rscen:SolarThermalFaçadeInstallation
  rdf:type rscen:RenoAlternative ;
  rscen:refines rscen:HotWaterReplacement ;
.
rscen:SolarThermalRoofInstallation
  rdf:type rscen:RenoAlternative ;
  rscen:refines rscen:HotWaterReplacement ;
.
rscen:TripleGlazedWindowInstallation
  rdf:type rscen:RenoAlternative ;
  rscen:refines rscen:WindowsReplacement ;
.
rscen:VentilationReplacement
  rdf:type rscen:RenoApproach ;
.
rscen:WaterAirHeatPumpInstallation
  rdf:type rscen:RenoAlternative ;
  rscen:refines rscen:CoolingInstallation ;
  rscen:refines rscen:HeatingInstallation ;
  rscen:refines rscen:HeatingReplacement ;
.
rscen:WaterWaterHeatPumpInstallation
  rdf:type rscen:RenoAlternative ;
  rscen:refines rscen:CoolingInstallation ;
  rscen:refines rscen:HeatingInstallation ;
  rscen:refines rscen:HeatingReplacement ;
  rscen:refines rscen:HotWaterReplacement ;
.
rscen:WindowGlazing
  rdf:type rscen:BuildingCharacteristics ;
  rdfs:comment "The type of glazing on the windows." ;
  rscen:value [
      owl:oneOf (
          "Simple"
          "Double"
          "Triple"
        ) ;
    ] ;
.
rscen:WindowsReplacement
  rdf:type rscen:RenoApproach ;
.
rscen:forProject
  rdf:type owl:ObjectProperty ;
  rdfs:domain rscen:Criterion ;
  rdfs:domain rscen:RenoScenario ;
  rdfs:isDefinedBy rscen: ;
  rdfs:range rscen:RenoProject ;
.
rscen:hasProperty
  rdf:type owl:ObjectProperty ;
.
rscen:isMadeOf
  rdf:type owl:ObjectProperty ;
  rdfs:domain rscen:RenoScenario ;
  rdfs:isDefinedBy rscen: ;
  rdfs:range rscen:RenoAction ;
.
rscen:nZeBScenario
  rdf:type owl:Class ;
  rdfs:subClassOf rscen:RenoScenario ;
.
rscen:refines
  rdf:type owl:ObjectProperty ;
  rdfs:domain rscen:RenoAlternative ;
  rdfs:domain rscen:RenoApproach ;
  rdfs:isDefinedBy rscen: ;
  rdfs:range rscen:RenoAction ;
  rdfs:range rscen:RenoAlternative ;
.
rscen:value
  rdf:type owl:DatatypeProperty ;
  rdfs:domain rscen:Criterion ;
.
<https://orcid.org/0000-0001-6085-8461>
  rdf:type vcard:Individual ;
  rdf:type schema:Person ;
  vcard:fn "Pierre Bourreau" ;
  schema:name "Pierre Bourreau" ;
.
schema:domainIncludes
  rdf:type owl:AnnotationProperty ;
.
schema:name
  rdf:type owl:AnnotationProperty ;
.
schema:rangeIncludes
  rdf:type owl:AnnotationProperty ;
.
